simplify Range.toList and add theorems

Lott/Data/Range.lean
@@ -1,14 +1,113 @@
 namespace Std.Range
 
-def toList (range : Range) : List Nat :=
-  let rec loop (fuel i stop step : Nat) : List Nat :=
-    if i ≥ stop then
-      []
-    else match fuel with
-     | 0 => []
-     | fuel + 1 => i :: loop fuel (i + step) stop step
-  loop range.stop range.start range.stop range.step
+def toList (r : Range) : List Nat := if r.step = 0 then
+   []
+  else if r.start < r.stop then
+    r.start :: toList { r with start := r.start + r.step }
+  else
+    []
 
 instance : Coe Range (List Nat) := ⟨Std.Range.toList⟩
+
+theorem toList_append (h₁ : l ≤ m) (h₂ : m ≤ n) : [l:m] ++ [m:n] = [l:n].toList := by
+  rw [toList, if_neg Nat.one_ne_zero]
+  split
+  · case isTrue h =>
+    apply Eq.symm
+    rw [toList, if_neg Nat.one_ne_zero]
+    apply Eq.symm
+    simp only at *
+    rw [if_pos (Nat.lt_of_lt_of_le h h₂), List.cons_append, toList_append (Nat.succ_le_of_lt h) h₂]
+  · case isFalse h =>
+    simp only at *
+    have : l = m := match Nat.lt_trichotomy l m with
+      | .inl lltm => h lltm |>.elim
+      | .inr (.inl leqm) => leqm
+      | .inr (.inr mltn) => Nat.not_lt_of_le h₁ mltn |>.elim
+    rw [this, List.nil_append]
+termination_by m - l
+decreasing_by
+  all_goals simp_wf
+  apply Nat.sub_succ_lt_self
+  assumption
+
+theorem toList_eq_nil_of_stop_le_start (h : r.stop ≤ r.start) : toList r = [] := by
+  rw [toList]
+  split
+  · case isTrue => rfl
+  · case isFalse => rw [if_neg (Nat.not_lt_of_le h)]
+
+theorem map_eq_of_eq_of_mem {f g : Nat → α} (h : ∀ i ∈ [m:n], f i = g i)
+  : List.map (fun i => f i) [m:n] = List.map (fun i => g i) [m:n] := by
+  rw [toList]
+  split
+  · case isTrue =>
+    contradiction
+  · case isFalse =>
+    split
+    · case isTrue => contradiction
+    · case isFalse =>
+      split
+      · case isTrue h' =>
+        simp only [List.map] at *
+        let h'' i (mem : i ∈ [m + 1:n]) := h i ⟨Nat.le_of_succ_le mem.lower, mem.upper⟩
+        rw [h m ⟨Nat.le_refl _, h'⟩, map_eq_of_eq_of_mem (m := m + 1) h'']
+      · case isFalse h => rfl
+termination_by n - m
+decreasing_by
+  all_goals simp_wf
+  apply Nat.sub_succ_lt_self
+  assumption
+
+theorem map_eq_of_eq_of_mem' {f g : Nat → α} (h : ∀ i ∈ [m:n], f i = g i)
+  : List.map (fun i => f i) (Coe.coe [m:n]) = List.map (fun i => g i) (Coe.coe [m:n]) := by
+  dsimp [Coe.coe]
+  exact map_eq_of_eq_of_mem h
+
+theorem mem_of_mem_map {f : Nat → α} (h : x ∈ List.map (fun i => f i) [m:n])
+  : ∃ i ∈ [m:n], x = f i := by
+  rw [toList, if_neg Nat.one_ne_zero] at h
+  split at h
+  · case isTrue h' =>
+    rw [List.map] at h
+    cases h
+    · case head => exact .intro m ⟨⟨Nat.le_refl _, h'⟩, rfl⟩
+    · case tail h'' =>
+      have ⟨i, mem, eq⟩ := mem_of_mem_map (m := m + 1) h''
+      exact ⟨i, ⟨Nat.le_of_succ_le mem.lower, mem.upper⟩, eq⟩
+  · case isFalse h' => cases h
+termination_by n - m
+decreasing_by
+  all_goals simp_wf
+  apply Nat.sub_succ_lt_self
+  assumption
+
+theorem map_shift {f : Nat → α} (h : j ≤ m)
+  : List.map (fun i => f (i + j)) [m - j:n - j] = List.map (fun i => f i) [m:n] := by
+  rw [toList]
+  apply Eq.symm
+  rw [toList]
+  apply Eq.symm
+  rw [if_neg Nat.one_ne_zero, if_neg Nat.one_ne_zero]
+  simp only
+  split
+  · case isTrue h' =>
+    rw [if_pos, List.map, Nat.sub_add_cancel h, ← Nat.sub_add_comm h, map_shift (m := m + 1),
+        ← List.map]
+    · exact Nat.le_succ_of_le h
+    · have := Nat.sub_pos_of_lt h'
+      rw [Nat.sub_right_comm, Nat.sub_sub, Nat.sub_add_cancel h] at this
+      exact Nat.lt_of_sub_pos this
+  · case isFalse h' =>
+    rw [List.map, if_neg, List.map]
+    intro h''
+    apply h'
+    have := Nat.sub_pos_of_lt h''
+    rw [← Nat.sub_add_cancel h, ← Nat.sub_sub, ← Nat.sub_right_comm] at this
+    exact Nat.lt_of_sub_pos this
+
+theorem map_append {f : Nat → α} (h₁ : l ≤ m) (h₂ : m ≤ n)
+  : List.map f [l:m] ++ List.map f [m:n] = List.map f [l:n] := by
+  rw [← List.map_append, toList_append h₁ h₂]
 
 end Std.Range
